cfrontend/Cshmgenproof.v
@@ -152,8 +152,8 @@ Qed.
 (** Transformation of expressions and statements. *)
 
 Lemma transl_expr_lvalue:
-  forall ge e le m a loc ofs ce ta,
-  Clight.eval_lvalue ge e le m a loc ofs ->
+  forall ge e c le m a loc ofs ce ta,
+  Clight.eval_lvalue ge e c le m a loc ofs ->
   transl_expr ce a = OK ta ->
   (exists tb, transl_lvalue ce a = OK tb /\ make_load tb (typeof a) = OK ta).
 Proof.
@@ -228,37 +228,40 @@ Variables cunit prog: Clight.program.
 Hypothesis LINK: linkorder cunit prog.
 Variable ge: genv.
 
+Section WithCp.
+Variable cp: compartment.
+
 Lemma make_intconst_correct:
   forall n e le m,
-  eval_expr ge e le m (make_intconst n) (Vint n).
+  eval_expr ge e cp le m (make_intconst n) (Vint n).
 Proof.
   intros. unfold make_intconst. econstructor. reflexivity.
 Qed.
 
 Lemma make_floatconst_correct:
   forall n e le m,
-  eval_expr ge e le m (make_floatconst n) (Vfloat n).
+  eval_expr ge e cp le m (make_floatconst n) (Vfloat n).
 Proof.
   intros. unfold make_floatconst. econstructor. reflexivity.
 Qed.
 
 Lemma make_singleconst_correct:
   forall n e le m,
-  eval_expr ge e le m (make_singleconst n) (Vsingle n).
+  eval_expr ge e cp le m (make_singleconst n) (Vsingle n).
 Proof.
   intros. unfold make_singleconst. econstructor. reflexivity.
 Qed.
 
 Lemma make_longconst_correct:
   forall n e le m,
-  eval_expr ge e le m (make_longconst n) (Vlong n).
+  eval_expr ge e cp le m (make_longconst n) (Vlong n).
 Proof.
   intros. unfold make_floatconst. econstructor. reflexivity.
 Qed.
 
 Lemma make_ptrofsconst_correct:
   forall n e le m,
-  eval_expr ge e le m (make_ptrofsconst n) (Vptrofs (Ptrofs.repr n)).
+  eval_expr ge e cp le m (make_ptrofsconst n) (Vptrofs (Ptrofs.repr n)).
 Proof.
   intros. unfold Vptrofs, make_ptrofsconst. destruct Archi.ptr64 eqn:SF.
 - replace (Ptrofs.to_int64 (Ptrofs.repr n)) with (Int64.repr n).
@@ -271,24 +274,24 @@ Qed.
 
 Lemma make_singleoffloat_correct:
   forall a n e le m,
-  eval_expr ge e le m a (Vfloat n) ->
-  eval_expr ge e le m (make_singleoffloat a) (Vsingle (Float.to_single n)).
+  eval_expr ge e cp le m a (Vfloat n) ->
+  eval_expr ge e cp le m (make_singleoffloat a) (Vsingle (Float.to_single n)).
 Proof.
   intros. econstructor. eauto. auto.
 Qed.
 
 Lemma make_floatofsingle_correct:
   forall a n e le m,
-  eval_expr ge e le m a (Vsingle n) ->
-  eval_expr ge e le m (make_floatofsingle a) (Vfloat (Float.of_single n)).
+  eval_expr ge e cp le m a (Vsingle n) ->
+  eval_expr ge e cp le m (make_floatofsingle a) (Vfloat (Float.of_single n)).
 Proof.
   intros. econstructor. eauto. auto.
 Qed.
 
 Lemma make_floatofint_correct:
   forall a n sg e le m,
-  eval_expr ge e le m a (Vint n) ->
-  eval_expr ge e le m (make_floatofint a sg) (Vfloat(cast_int_float sg n)).
+  eval_expr ge e cp le m a (Vint n) ->
+  eval_expr ge e cp le m (make_floatofint a sg) (Vfloat(cast_int_float sg n)).
 Proof.
   intros. unfold make_floatofint, cast_int_float.
   destruct sg; econstructor; eauto.
@@ -302,12 +305,12 @@ Hint Extern 2 (@eq trace _ _) => traceEq: cshm.
 
 Lemma make_cmpu_ne_zero_correct:
   forall e le m a n,
-  eval_expr ge e le m a (Vint n) ->
-  eval_expr ge e le m (make_cmpu_ne_zero a) (Vint (if Int.eq n Int.zero then Int.zero else Int.one)).
+  eval_expr ge e cp le m a (Vint n) ->
+  eval_expr ge e cp le m (make_cmpu_ne_zero a) (Vint (if Int.eq n Int.zero then Int.zero else Int.one)).
 Proof.
   intros.
-  assert (DEFAULT: eval_expr ge e le m (Ebinop (Ocmpu Cne) a (make_intconst Int.zero))
-                                       (Vint (if Int.eq n Int.zero then Int.zero else Int.one))).
+  assert (DEFAULT: eval_expr ge e cp le m (Ebinop (Ocmpu Cne) a (make_intconst Int.zero))
+                             (Vint (if Int.eq n Int.zero then Int.zero else Int.one))).
   { econstructor; eauto with cshm. simpl. unfold Val.cmpu, Val.cmpu_bool.
     unfold Int.cmpu. destruct (Int.eq n Int.zero); auto. }
   assert (CMP: forall ob,
@@ -335,13 +338,13 @@ Qed.
 
 Lemma make_cmpu_ne_zero_correct_ptr:
   forall e le m a b i,
-  eval_expr ge e le m a (Vptr b i) ->
+  eval_expr ge e cp le m a (Vptr b i) ->
   Archi.ptr64 = false ->
   Mem.weak_valid_pointer m b (Ptrofs.unsigned i) = true ->
-  eval_expr ge e le m (make_cmpu_ne_zero a) Vone.
+  eval_expr ge e cp le m (make_cmpu_ne_zero a) Vone.
 Proof.
   intros.
-  assert (DEFAULT: eval_expr ge e le m (Ebinop (Ocmpu Cne) a (make_intconst Int.zero)) Vone).
+  assert (DEFAULT: eval_expr ge e cp le m (Ebinop (Ocmpu Cne) a (make_intconst Int.zero)) Vone).
   { econstructor; eauto with cshm. simpl. unfold Val.cmpu, Val.cmpu_bool.
     unfold Mem.weak_valid_pointer in H1. rewrite H0, H1.
     rewrite Int.eq_true; auto. }
@@ -360,8 +363,8 @@ Qed.
 
 Lemma make_cast_int_correct:
   forall e le m a n sz si,
-  eval_expr ge e le m a (Vint n) ->
-  eval_expr ge e le m (make_cast_int a sz si) (Vint (cast_int_int sz si n)).
+  eval_expr ge e cp le m a (Vint n) ->
+  eval_expr ge e cp le m (make_cast_int a sz si) (Vint (cast_int_int sz si n)).
 Proof.
   intros. unfold make_cast_int, cast_int_int.
   destruct sz.
@@ -373,8 +376,8 @@ Qed.
 
 Lemma make_longofint_correct:
   forall e le m a n si,
-  eval_expr ge e le m a (Vint n) ->
-  eval_expr ge e le m (make_longofint a si) (Vlong (cast_int_long si n)).
+  eval_expr ge e cp le m a (Vint n) ->
+  eval_expr ge e cp le m (make_longofint a si) (Vlong (cast_int_long si n)).
 Proof.
   intros. unfold make_longofint, cast_int_long. destruct si; eauto with cshm.
 Qed.
@@ -393,9 +396,9 @@ Ltac InvEval :=
 Lemma make_cast_correct:
   forall e le m a b v ty1 ty2 v',
   make_cast ty1 ty2 a = OK b ->
-  eval_expr ge e le m a v ->
+  eval_expr ge e cp le m a v ->
   sem_cast v ty1 ty2 m = Some v' ->
-  eval_expr ge e le m b v'.
+  eval_expr ge e cp le m b v'.
 Proof.
   intros. unfold make_cast, sem_cast in *;
   destruct (classify_cast ty1 ty2); inv H; destruct v; InvEval; eauto with cshm.
@@ -447,10 +450,10 @@ Qed.
 
 Lemma make_boolean_correct:
  forall e le m a v ty b,
-  eval_expr ge e le m a v ->
+  eval_expr ge e cp le m a v ->
   bool_val v ty m = Some b ->
   exists vb,
-    eval_expr ge e le m (make_boolean a ty) vb
+    eval_expr ge e cp le m (make_boolean a ty) vb
     /\ Val.bool_of_val vb b.
 Proof.
   intros. unfold make_boolean. unfold bool_val in H0.
@@ -482,8 +485,8 @@ Lemma make_neg_correct:
   forall a tya c va v e le m,
   sem_neg va tya = Some v ->
   make_neg a tya = OK c ->
-  eval_expr ge e le m a va ->
-  eval_expr ge e le m c v.
+  eval_expr ge e cp le m a va ->
+  eval_expr ge e cp le m c v.
 Proof.
   unfold sem_neg, make_neg; intros until m; intros SEM MAKE EV1;
   destruct (classify_neg tya); inv MAKE; destruct va; inv SEM; eauto with cshm.
@@ -493,8 +496,8 @@ Lemma make_absfloat_correct:
   forall a tya c va v e le m,
   sem_absfloat va tya = Some v ->
   make_absfloat a tya = OK c ->
-  eval_expr ge e le m a va ->
-  eval_expr ge e le m c v.
+  eval_expr ge e cp le m a va ->
+  eval_expr ge e cp le m c v.
 Proof.
   unfold sem_absfloat, make_absfloat; intros until m; intros SEM MAKE EV1;
   destruct (classify_neg tya); inv MAKE; destruct va; inv SEM; eauto with cshm.
@@ -507,8 +510,8 @@ Lemma make_notbool_correct:
   forall a tya c va v e le m,
   sem_notbool va tya m = Some v ->
   make_notbool a tya = OK c ->
-  eval_expr ge e le m a va ->
-  eval_expr ge e le m c v.
+  eval_expr ge e cp le m a va ->
+  eval_expr ge e cp le m c v.
 Proof.
   unfold sem_notbool, bool_val, make_notbool; intros until m; intros SEM MAKE EV1.
   destruct (classify_bool tya); inv MAKE; destruct va; simpl in SEM; InvEval.
@@ -534,8 +537,8 @@ Lemma make_notint_correct:
   forall a tya c va v e le m,
   sem_notint va tya = Some v ->
   make_notint a tya = OK c ->
-  eval_expr ge e le m a va ->
-  eval_expr ge e le m c v.
+  eval_expr ge e cp le m a va ->
+  eval_expr ge e cp le m c v.
 Proof.
   unfold sem_notint, make_notint; intros until m; intros SEM MAKE EV1;
   destruct (classify_notint tya); inv MAKE; destruct va; inv SEM; eauto with cshm.
@@ -547,9 +550,9 @@ Definition binary_constructor_correct
   forall a tya b tyb c va vb v e le m,
   sem va tya vb tyb m = Some v ->
   make a tya b tyb = OK c ->
-  eval_expr ge e le m a va ->
-  eval_expr ge e le m b vb ->
-  eval_expr ge e le m c v.
+  eval_expr ge e cp le m a va ->
+  eval_expr ge e cp le m b vb ->
+  eval_expr ge e cp le m c v.
 
 Definition shift_constructor_correct
     (make: expr -> type -> expr -> type -> res expr)
@@ -557,9 +560,9 @@ Definition shift_constructor_correct
   forall a tya b tyb c va vb v e le m,
   sem va tya vb tyb = Some v ->
   make a tya b tyb = OK c ->
-  eval_expr ge e le m a va ->
-  eval_expr ge e le m b vb ->
-  eval_expr ge e le m c v.
+  eval_expr ge e cp le m a va ->
+  eval_expr ge e cp le m b vb ->
+  eval_expr ge e cp le m c v.
 
 Section MAKE_BIN.
 
@@ -634,9 +637,9 @@ Lemma make_add_correct: binary_constructor_correct (make_add cunit.(prog_comp_en
 Proof.
   assert (A: forall ty si a b c e le m va vb v,
              make_add_ptr_int cunit.(prog_comp_env) ty si a b = OK c ->
-             eval_expr ge e le m a va -> eval_expr ge e le m b vb ->
+             eval_expr ge e cp le m a va -> eval_expr ge e cp le m b vb ->
              sem_add_ptr_int (prog_comp_env prog) ty si va vb = Some v ->
-             eval_expr ge e le m c v).
+             eval_expr ge e cp le m c v).
   { unfold make_add_ptr_int, sem_add_ptr_int; intros until v; intros MAKE EV1 EV2 SEM; monadInv MAKE.
     destruct Archi.ptr64 eqn:SF; inv EQ0; rewrite (transl_sizeof _ _ _ _ LINK EQ).
   - destruct va; InvEval; destruct vb; inv SEM.
@@ -655,9 +658,9 @@ Proof.
   }
   assert (B: forall ty a b c e le m va vb v,
              make_add_ptr_long cunit.(prog_comp_env) ty a b = OK c ->
-             eval_expr ge e le m a va -> eval_expr ge e le m b vb ->
+             eval_expr ge e cp le m a va -> eval_expr ge e cp le m b vb ->
              sem_add_ptr_long (prog_comp_env prog) ty va vb = Some v ->
-             eval_expr ge e le m c v).
+             eval_expr ge e cp le m c v).
   { unfold make_add_ptr_long, sem_add_ptr_long; intros until v; intros MAKE EV1 EV2 SEM; monadInv MAKE.
     destruct Archi.ptr64 eqn:SF; inv EQ0; rewrite (transl_sizeof _ _ _ _ LINK EQ).
   - destruct va; InvEval; destruct vb; inv SEM.
@@ -855,9 +858,9 @@ Qed.
 Lemma make_cmp_ptr_correct:
   forall cmp e le m a va b vb v,
   cmp_ptr m cmp va vb = Some v ->
-  eval_expr ge e le m a va ->
-  eval_expr ge e le m b vb ->
-  eval_expr ge e le m (make_cmp_ptr cmp a b) v.
+  eval_expr ge e cp le m a va ->
+  eval_expr ge e cp le m b vb ->
+  eval_expr ge e cp le m (make_cmp_ptr cmp a b) v.
 Proof.
   unfold cmp_ptr, make_cmp_ptr; intros.
   destruct Archi.ptr64.
@@ -868,8 +871,8 @@ Qed.
 
 Remark make_ptrofs_of_int_correct:
   forall e le m a i si,
-  eval_expr ge e le m a (Vint i) ->
-  eval_expr ge e le m (if Archi.ptr64 then make_longofint a si else a) (Vptrofs (ptrofs_of_int si i)).
+  eval_expr ge e cp le m a (Vint i) ->
+  eval_expr ge e cp le m (if Archi.ptr64 then make_longofint a si else a) (Vptrofs (ptrofs_of_int si i)).
 Proof.
   intros. unfold Vptrofs, ptrofs_of_int. destruct Archi.ptr64 eqn:SF.
 - unfold make_longofint. destruct si.
@@ -888,8 +891,8 @@ Qed.
 
 Remark make_ptrofs_of_int64_correct:
   forall e le m a i,
-  eval_expr ge e le m a (Vlong i) ->
-  eval_expr ge e le m (if Archi.ptr64 then a else Eunop Ointoflong a) (Vptrofs (Ptrofs.of_int64 i)).
+  eval_expr ge e cp le m a (Vlong i) ->
+  eval_expr ge e cp le m (if Archi.ptr64 then a else Eunop Ointoflong a) (Vptrofs (Ptrofs.of_int64 i)).
 Proof.
   intros. unfold Vptrofs. destruct Archi.ptr64 eqn:SF.
 - replace (Ptrofs.to_int64 (Ptrofs.of_int64 i)) with i. auto.
@@ -914,8 +917,8 @@ Lemma transl_unop_correct:
   forall op a tya c va v e le m,
   transl_unop op a tya = OK c ->
   sem_unary_operation op va tya m = Some v ->
-  eval_expr ge e le m a va ->
-  eval_expr ge e le m c v.
+  eval_expr ge e cp le m a va ->
+  eval_expr ge e cp le m c v.
 Proof.
   intros. destruct op; simpl in *.
   eapply make_notbool_correct; eauto.
@@ -928,9 +931,9 @@ Lemma transl_binop_correct:
   forall op a tya b tyb c va vb v e le m,
   transl_binop cunit.(prog_comp_env) op a tya b tyb = OK c ->
   sem_binary_operation prog.(prog_comp_env) op va tya vb tyb m = Some v ->
-  eval_expr ge e le m a va ->
-  eval_expr ge e le m b vb ->
-  eval_expr ge e le m c v.
+  eval_expr ge e cp le m a va ->
+  eval_expr ge e cp le m b vb ->
+  eval_expr ge e cp le m c v.
 Proof.
   intros. destruct op; simpl in *.
   eapply make_add_correct; eauto.
@@ -951,12 +954,14 @@ Proof.
   eapply make_cmp_correct; eauto.
 Qed.
 
+End WithCp.
+
 Lemma make_load_correct:
-  forall addr ty code b ofs v e le m,
+  forall cp addr ty code b ofs v e le m,
   make_load addr ty = OK code ->
-  eval_expr ge e le m addr (Vptr b ofs) ->
-  deref_loc ty m b ofs v ->
-  eval_expr ge e le m code v.
+  eval_expr ge e cp le m addr (Vptr b ofs) ->
+  deref_loc cp ty m b ofs v ->
+  eval_expr ge e cp le m code v.
 Proof.
   unfold make_load; intros until m; intros MKLOAD EVEXP DEREF.
   inv DEREF.
@@ -970,9 +975,9 @@ Qed.
 
 Lemma make_memcpy_correct:
   forall f dst src ty k e le m b ofs v m' s,
-  eval_expr ge e le m dst (Vptr b ofs) ->
-  eval_expr ge e le m src v ->
-  assign_loc prog.(prog_comp_env) ty m b ofs v m' ->
+  eval_expr ge e (comp_of f) le m dst (Vptr b ofs) ->
+  eval_expr ge e (comp_of f) le m src v ->
+  assign_loc prog.(prog_comp_env) (comp_of f) ty m b ofs v m' ->
   access_mode ty = By_copy ->
   make_memcpy cunit.(prog_comp_env) dst src ty = OK s ->
   step ge (State f s k e le m) E0 (State f Sskip k e le m').
@@ -982,7 +987,8 @@ Proof.
   exploit transl_alignof_blockcopy. eexact LINK. eauto. intros [A B]. rewrite A, B.
   change le with (set_optvar None Vundef le) at 2.
   econstructor.
-  econstructor. eauto. econstructor. eauto. constructor.
+  econstructor.
+  eauto. econstructor. eauto. constructor.
   econstructor; eauto.
   apply alignof_blockcopy_1248.
   apply sizeof_pos.
@@ -992,9 +998,9 @@ Qed.
 Lemma make_store_correct:
   forall addr ty rhs code e le m b ofs v m' f k,
   make_store cunit.(prog_comp_env) addr ty rhs = OK code ->
-  eval_expr ge e le m addr (Vptr b ofs) ->
-  eval_expr ge e le m rhs v ->
-  assign_loc prog.(prog_comp_env) ty m b ofs v m' ->
+  eval_expr ge e (comp_of f) le m addr (Vptr b ofs) ->
+  eval_expr ge e (comp_of f) le m rhs v ->
+  assign_loc prog.(prog_comp_env) (comp_of f) ty m b ofs v m' ->
   step ge (State f code k e le m) E0 (State f Sskip k e le m').
 Proof.
   unfold make_store. intros until k; intros MKSTORE EV1 EV2 ASSIGN.
@@ -1008,10 +1014,10 @@ Proof.
 Qed.
 
 Lemma make_normalization_correct:
-  forall e le m a v t,
-  eval_expr ge e le m a v ->
+  forall e cp le m a v t,
+  eval_expr ge e cp le m a v ->
   wt_val v t ->
-  eval_expr ge e le m (make_normalization t a) v.
+  eval_expr ge e cp le m (make_normalization t a) v.
 Proof.
   intros. destruct t; simpl; auto. inv H0.
 - destruct i; simpl in H3.
@@ -1125,10 +1131,10 @@ Proof.
 Qed.
 
 Lemma match_env_free_blocks:
-  forall e te m m',
+  forall e cp te m m',
   match_env e te ->
-  Mem.free_list m (Clight.blocks_of_env ge e) = Some m' ->
-  Mem.free_list m (blocks_of_env te) = Some m'.
+  Mem.free_list m (Clight.blocks_of_env ge e) cp = Some m' ->
+  Mem.free_list m (blocks_of_env te) cp = Some m'.
 Proof.
   intros. rewrite (match_env_same_blocks _ _ H). auto.
 Qed.
@@ -1148,12 +1154,12 @@ Qed.
 
 Lemma match_env_alloc_variables:
   forall cunit, linkorder cunit prog ->
-  forall e1 m1 vars e2 m2, Clight.alloc_variables ge e1 m1 vars e2 m2 ->
+  forall cp e1 m1 vars e2 m2, Clight.alloc_variables ge cp e1 m1 vars e2 m2 ->
   forall tvars te1,
   mmap (transl_var cunit.(prog_comp_env)) vars = OK tvars ->
   match_env e1 te1 ->
   exists te2,
-  Csharpminor.alloc_variables te1 m1 tvars te2 m2
+  Csharpminor.alloc_variables cp te1 m1 tvars te2 m2
   /\ match_env e2 te2.
 Proof.
   induction 2; simpl; intros.
@@ -1234,16 +1240,17 @@ Variable le: temp_env.
 Variable m: mem.
 Variable te: Csharpminor.env.
 Hypothesis MENV: match_env e te.
+Variable cp: compartment.
 
 Lemma transl_expr_lvalue_correct:
   (forall a v,
-   Clight.eval_expr ge e le m a v ->
+   Clight.eval_expr ge e cp le m a v ->
    forall ta (TR: transl_expr cunit.(prog_comp_env) a = OK ta) ,
-   Csharpminor.eval_expr tge te le m ta v)
+   Csharpminor.eval_expr tge te cp le m ta v)
 /\(forall a b ofs,
-   Clight.eval_lvalue ge e le m a b ofs ->
+   Clight.eval_lvalue ge e cp le m a b ofs ->
    forall ta (TR: transl_lvalue cunit.(prog_comp_env) a = OK ta),
-   Csharpminor.eval_expr tge te le m ta (Vptr b ofs)).
+   Csharpminor.eval_expr tge te cp le m ta (Vptr b ofs)).
 Proof.
   apply eval_expr_lvalue_ind; intros; try (monadInv TR).
 - (* const int *)
@@ -1299,23 +1306,23 @@ Qed.
 
 Lemma transl_expr_correct:
    forall a v,
-   Clight.eval_expr ge e le m a v ->
+   Clight.eval_expr ge e cp le m a v ->
    forall ta, transl_expr cunit.(prog_comp_env) a = OK ta ->
-   Csharpminor.eval_expr tge te le m ta v.
+   Csharpminor.eval_expr tge te cp le m ta v.
 Proof (proj1 transl_expr_lvalue_correct).
 
 Lemma transl_lvalue_correct:
    forall a b ofs,
-   Clight.eval_lvalue ge e le m a b ofs ->
+   Clight.eval_lvalue ge e cp le m a b ofs ->
    forall ta, transl_lvalue cunit.(prog_comp_env) a = OK ta ->
-   Csharpminor.eval_expr tge te le m ta (Vptr b ofs).
+   Csharpminor.eval_expr tge te cp le m ta (Vptr b ofs).
 Proof (proj2 transl_expr_lvalue_correct).
 
 Lemma transl_arglist_correct:
   forall al tyl vl,
-  Clight.eval_exprlist ge e le m al tyl vl ->
+  Clight.eval_exprlist ge e cp le m al tyl vl ->
   forall tal, transl_arglist cunit.(prog_comp_env) al tyl = OK tal ->
-  Csharpminor.eval_exprlist tge te le m tal vl.
+  Csharpminor.eval_exprlist tge te cp le m tal vl.
 Proof.
   induction 1; intros.
   monadInv H. constructor.
@@ -1325,7 +1332,7 @@ Qed.
 
 Lemma typlist_of_arglist_eq:
   forall al tyl vl,
-  Clight.eval_exprlist ge e le m al tyl vl ->
+  Clight.eval_exprlist ge e cp le m al tyl vl ->
   typlist_of_arglist al tyl = typlist_of_typelist tyl.
 Proof.
   induction 1; simpl.
@@ -1409,7 +1416,7 @@ Inductive match_cont: composite_env -> type -> nat -> nat -> Clight.cont -> Csha
       transl_function cu.(prog_comp_env) f = OK tf ->
       match_env e te ->
       match_cont cu.(prog_comp_env) (Clight.fn_return f) nbrk' ncnt' k tk ->
-      (forall v e le m, wt_val v tyret -> le!id = Some v -> eval_expr tge e le m a v) ->
+      (forall v e le m, wt_val v tyret -> le!id = Some v -> eval_expr tge e (comp_of f) le m a v) ->
       match_cont ce tyret nbrk ncnt
                  (Clight.Kcall (Some id) f e le k)
                  (Kcall (Some id) tf te le (Kseq (Sset id a) tk)).
@@ -1610,13 +1617,18 @@ Proof.
   destruct SAME; subst ts' tk'.
   econstructor; split.
   apply plus_one. eapply make_store_correct; eauto.
-  eapply transl_lvalue_correct; eauto. eapply make_cast_correct; eauto.
+  rewrite <- (comp_transl_function _ _ _ TRF).
+  eapply transl_lvalue_correct; eauto.
+  rewrite <- (comp_transl_function _ _ _ TRF).
+  eapply make_cast_correct; eauto.
   eapply transl_expr_correct; eauto.
+  rewrite <- (comp_transl_function _ _ _ TRF). eauto.
   eapply match_states_skip; eauto.
 
 - (* set *)
   monadInv TR. inv MTR. econstructor; split.
   apply plus_one. econstructor. eapply transl_expr_correct; eauto.
+  rewrite <- (comp_transl_function _ _ _ TRF). eauto.
   eapply match_states_skip; eauto.
 
 - (* call *)
@@ -1644,7 +1656,9 @@ Proof.
     econstructor; split.
     apply plus_one. eapply step_call; eauto.
     eapply transl_expr_correct with (cunit := cu); eauto.
+    rewrite <- (comp_transl_function _ _ _ TRF). eauto.
     eapply transl_arglist_correct with (cunit := cu); eauto.
+    rewrite <- (comp_transl_function _ _ _ TRF). eauto.
     eapply allowed_call_translated; eauto.
     econstructor; eauto.
     eapply match_Kcall with (ce := prog_comp_env cu') (cu := cu); eauto.
@@ -1654,7 +1668,9 @@ Proof.
     econstructor; split.
     eapply plus_two. apply step_seq. eapply step_call; eauto. 
     eapply transl_expr_correct with (cunit := cu); eauto.
+    rewrite <- (comp_transl_function _ _ _ TRF). eauto.
     eapply transl_arglist_correct with (cunit := cu); eauto.
+    rewrite <- (comp_transl_function _ _ _ TRF). eauto.
     eapply allowed_call_translated; eauto.
     traceEq.
     econstructor; eauto.
@@ -1667,6 +1683,7 @@ Proof.
   econstructor; split.
   apply plus_one. econstructor.
   eapply transl_arglist_correct; eauto.
+  rewrite <- (comp_transl_function _ _ _ TRF). eauto.
   eapply external_call_symbols_preserved with (ge1 := ge). apply senv_preserved. eauto.
   change tf.(fn_comp) with (comp_of tf). now rewrite <- (comp_transl_partial _ TRF); eauto.
   eapply match_states_skip; eauto.
@@ -1703,6 +1720,7 @@ Proof.
   intros [v [A B]].
   econstructor; split.
   apply plus_one. apply step_ifthenelse with (v := v) (b := b); auto.
+  rewrite <- (comp_transl_function _ _ _ TRF). eauto.
   destruct b; econstructor; eauto; constructor.
 
 - (* loop *)
@@ -1756,6 +1774,7 @@ Proof.
   econstructor; split.
   apply plus_one. constructor.
   eapply match_env_free_blocks; eauto.
+  rewrite <- (comp_transl_function _ _ _ TRF). eauto.
   eapply match_returnstate with (ce := prog_comp_env cu); eauto.
   eapply match_cont_call_cont. eauto.
   constructor.
@@ -1765,7 +1784,9 @@ Proof.
   econstructor; split.
   apply plus_one. constructor.
   eapply make_cast_correct; eauto. eapply transl_expr_correct; eauto.
+  rewrite <- (comp_transl_function _ _ _ TRF). eauto.
   eapply match_env_free_blocks; eauto.
+  rewrite <- (comp_transl_function _ _ _ TRF). eauto.
   eapply match_returnstate with (ce := prog_comp_env cu); eauto.
   eapply match_cont_call_cont. eauto.
   apply wt_val_casted. eapply cast_val_is_casted; eauto.
@@ -1776,6 +1797,7 @@ Proof.
   econstructor; split.
   apply plus_one. apply step_skip_call. auto.
   eapply match_env_free_blocks; eauto.
+  rewrite <- (comp_transl_function _ _ _ TRF). eauto.
   eapply match_returnstate with (ce := prog_comp_env cu); eauto.
   constructor.
 
@@ -1790,6 +1812,7 @@ Proof.
   econstructor; split.
   eapply star_plus_trans. eapply match_transl_step; eauto.
   apply plus_one. econstructor; eauto. traceEq.
+  rewrite <- (comp_transl_function _ _ _ TRF). eauto. eauto.
   econstructor; eauto.
   apply transl_lbl_stmt_2. apply transl_lbl_stmt_1. eauto.
   constructor.
@@ -1866,7 +1889,8 @@ Proof.
   + (* with normalization *)
     econstructor; split.
     eapply plus_three. econstructor. econstructor. constructor.
-    simpl. apply H13. eauto. apply PTree.gss.
+    simpl.
+    rewrite <- (comp_transl_function _ _ _ H10). apply H13. eauto. apply PTree.gss.
     traceEq.
     simpl. rewrite PTree.set2. econstructor; eauto. simpl; reflexivity. constructor.
 Qed.
